feat: Simpler first-order implementation for pure `SPred`s (#9841)
This PR migrates the ⌜p⌝ notation for embedding pure p : Prop into SPred
σs to expand into a simple, first-order expression SPred.pure p that can
be supported by e-matching in grind.

Doing so deprives ⌜p⌝ notation of its idiom-bracket-like support for
#selector and ‹Nat›ₛ syntax which is thus removed.

src/Std/Do/SPred/SVal.lean
@@ -24,9 +24,10 @@ namespace Std.Do
 abbrev SVal (σs : List (Type u)) (α : Type u) : Type u := match σs with
   | [] => α
   | σ :: σs => σ → SVal σs α
+
 /- Note about the reducibility of SVal:
 We need SVal to be reducible, otherwise type inference fails for `Triple`.
-(Begs for investigation. #8074.)
+This is tracked in #8074. There is a fix in #9015, but it regresses Mathlib.
 -/
 
 namespace SVal
@@ -59,22 +60,19 @@ def uncurry {σs : List (Type u)} (f : SVal σs α) : StateTuple σs → α := m
 @[simp, grind =] theorem uncurry_curry {σs : List (Type u)} {f : StateTuple σs → α} : uncurry (σs:=σs) (curry f) = f := by induction σs <;> (simp[uncurry, curry, *]; rfl)
 @[simp, grind =] theorem curry_uncurry {σs : List (Type u)} {f : SVal σs α} : curry (σs:=σs) (uncurry f) = f := by induction σs <;> simp[uncurry, curry, *]
 
-/-- Embed a pure value into an `SVal`. -/
-abbrev pure {σs : List (Type u)} (a : α) : SVal σs α := curry (fun _ => a)
-
 instance [Inhabited α] : Inhabited (SVal σs α) where
-  default := pure default
+  default := curry fun _ => default
 
 class GetTy (σ : Type u) (σs : List (Type u)) where
   get : SVal σs σ
 
 instance : GetTy σ (σ :: σs) where
-  get := fun s => pure s
+  get := fun s => curry (fun _ => s)
 
 instance [GetTy σ₁ σs] : GetTy σ₁ (σ₂ :: σs) where
   get := fun _ => GetTy.get
 
 /-- Get the top-most state of type `σ` from an `SVal`. -/
 def getThe {σs : List (Type u)} (σ : Type u) [GetTy σ σs] : SVal σs σ := GetTy.get
-@[simp, grind =] theorem getThe_here {σs : List (Type u)} (σ : Type u) (s : σ) : getThe (σs := σ::σs) σ s = pure s := rfl
+@[simp, grind =] theorem getThe_here {σs : List (Type u)} (σ : Type u) (s : σ) : getThe (σs := σ::σs) σ s = curry (fun _ => s) := rfl
 @[simp, grind =] theorem getThe_there {σs : List (Type u)} [GetTy σ σs] (σ' : Type u) (s : σ') : getThe (σs := σ'::σs) σ s = getThe (σs := σs) σ := rfl
